---
title: "Proof that r! divides product of r consecutive integers"
date: 2025-02-11
difficulty: Intermediate
tags: ["Number Theory"]
concepts: ["Mathematical Induction"]
equations:
  - $\displaystyle\binom{n+r}{r}$
categories: "Number Theory"
---

# Problem Statement
Prove that the product of any $r$ consecutive integers is divisible by $r!$, i.e.,
$$P(n,r):r!\mid n(n+1)\dots (n+r-1)$$
is true $\forall n,r\in\mathbb{N}$

# Preliminary Analysis
Denote
$$p(n,r):=n(n+1)(n+2)\dots(n+r-1)$$
Then, we have
$$
\begin{array}{rrl}
&p(n,r+1)&=n(n+1)(n+2)\dots(n+r-1)(n+r)\newline
\implies&p(n,r+1)&=n(n+1)(n+2)\dots(n+r-1)[(n-1)+(r+1)]\newline
&&=(n-1)n(n+1)(n+2)\dots(n+r-1)+(r+1)n(n+1)(n+2)\dots(n+r-1)\newline
&&=p(n-1,r+1)+(r+1)p(n,r)
\end{array}
$$

Hence, we have
$$p(n,r+1)=p(n-1,r+1)+(r+1)p(n,r)$$

Now, we have writing for $n$ from $n$ to $2$ and adding the following equations
$$
\begin{align*}
p(n,r+1)&=\bcancel{p(n-1,r+1)}+(r+1)p(n,r)\newline
\bcancel{p(n-1,r+1)}&=\bcancel{p(n-2,r+1)}+(r+1)p(n-1,r)\newline
\bcancel{p(n-2,r+1)}&=\bcancel{p(n-3,r+1)}+(r+1)p(n-2,r)\newline
\vdots&=\vdots+\vdots\newline
\bcancel{p(3,r+1)}&=\bcancel{p(2,r+1)}+(r+1)p(3,r)\newline
\bcancel{p(2,r+1)}&=p(1,r+1)+(r+1)p(2,r)\newline
\end{align*}
$$
we get
$$p(n,r+1)=p(1,r+1)+(r+1)[p(n,r)+p(n-1,r)+p(n-2,r)+\dots+p(3,r)+p(2,r)]$$
Since $p(1,r+1)=1\cdot2\cdot3\cdot\dots\cdot r\cdot(r+1)=(r+1)!$, we have
$$p(n,r+1)=(r+1)!+(r+1)[p(n,r)+p(n-1,r)+p(n-2,r)+\dots+p(3,r)+p(2,r)]$$

Now, for the second part, we have
$$
\begin{array}{rrl}
&p(n+1,r)&=(n+1)(n+2)(n+3)\dots(n+r-1)(n+r)\newline
\implies&p(n+1,r)&=n(n+1)(n+2)\dots(n+r-1)+r(n+1)(n+2)(n+3)\dots(n+r-1)\newline
&&=p(n,r)+rp(n+1,r-1)
\end{array}
$$

Hence, we have
$$p(n+1,r)=p(n,r)+rp(n+1,r-1)$$
Now, we have writing for $r$ from $r$ to $2$, we have following equations:
$$
\begin{array}{rlr}
p(n+1,r)&=p(n,r)+rp(n+1,r-1)&(1)\newline
p(n+1,r-1)&=p(n,r-1)+(r-1)p(n+1,r-2)&(2)\newline
p(n+1,r-2)&=p(n,r-2)+(r-2)p(n+1,r-3)&(3)\newline
\vdots&=\vdots+\vdots&\newline
p(n+1,3)&=p(n,3)+3p(n+1,2)&(r-2)\newline
p(n+1,2)&=p(n,2)+2p(n+1,1)&(r-1)\newline
\end{array}
$$
(1)+$r$(2)+$r(r-1)$(3)+\dots+$[r(r-1)\dots4]$(r-2)+$[r(r-1)\dots3]$(r-1)$\implies$
$$
\begin{align*}
p(n+1,r)&=p(n,r)+\bcancel{rp(n+1,r-1)}\newline
\bcancel{rp(n+1,r-1)}&=rp(n,r-1)+\bcancel{r(r-1)p(n+1,r-2)}\newline
\bcancel{r(r-1)p(n+1,r-2)}&=r(r-1)p(n,r-2)+\bcancel{r(r-1)(r-2)p(n+1,r-3)}\newline
\vdots&=\vdots+\vdots\newline
\bcancel{[r(r-1)\dots4]p(n+1,3)}&=[r(r-1)\dots4]p(n,3)+\bcancel{[r(r-1)\dots4]3p(n+1,2)}\newline
\bcancel{[r(r-1)\dots3]p(n+1,2)}&=[r(r-1)\dots3]p(n,2)+[r(r-1)\dots3]2p(n+1,1)
\end{align*}
$$
$\implies$
$$
\begin{array}{rl}
p(n+1,r)&=p(n,r)+rp(n,r-1)+r(r-1)p(n,r-2)+\dots+\newline
&[r(r-1)\dots4]p(n,3)[r(r-1)\dots3]p(n,2)+[r(r-1)\dots3]2p(n+1,1)
\end{array}
$$
Since $[r(r-1)\dots3]\cdot2=r!$ and $p(n+1,1)=(n+1)$, we have
$$p(n+1,r)=p(n,r)+\left\\{\sum_{i=2}^{r-1}\left[\prod_{j=0}^{(r-1)-i}(r-j)\right]p(n,i)\right\\}+(n+1)r!$$
Hence, we have two results
1. Result 1:$$p(n,r+1)=(r+1)!+(r+1)[p(n,r)+p(n-1,r)+p(n-2,r)+\dots+p(3,r)+p(2,r)]$$
2. Result 2:$$p(n+1,r)=p(n,r)+\left\\{{\sum_{i=2}^{r-1}\left[\prod_{j=0}^{(r-1)-i}(r-j)\right]p(n,i)}\right\\}+(n+1)r!$$
### Result 1
Suppose $r!\mid p(n,r)$ for $n\leq k$. Then, from result 1, since $p(k,r+1)=(r+1)!+(r+1)\cdot r!\cdot x=(r+1)!(1+x)$ for some $x\in\mathbb{N}$, we have $(r+1)!\mid p(k,r+1)$.
Hence, $$r!\mid p(n,r)\text{ for }n\leq k \implies (r+1)!\mid p(k,r+1)$$
### Result 2
Suppose $r!\mid p(n,r)$ for $r\leq u$. Then, from result 1, since $p(n+1,u)=p(n,u)+\displaystyle{\left\\{\sum_{i=2}^{u-1}\left[\prod_{j=0}^{(u-1)-i}(u-j)\right]p(n,i)\right\\}}+(n+1)u!$ and $p(n,i)=i!x_i$ for some $x_i\in\mathbb{N}$ we have, $u(u-1)\dots(i+1)p(n,i)=u!x_i$. Also, since $p(n,u)=u!x$ for some $x\in\mathbb{N}$, we have
$$
p(n+1,u)=u!x+\displaystyle{\left\\{\sum_{i=2}^{u-1}u!x_i\right\\}}+(n+1)u!s
$$
Hence, $u!\mid p(n+1,u)$.
Thus,
$$r!\mid p(n,r)\text{ for }r\leq u \implies u!\mid p(n+1,u)$$

# Results

Thus, we have two main results

1. Result 1$$r!\mid p(n,r)\text{ for }n\leq k \implies (r+1)!\mid p(k,r+1)$$
2. Result 2$$r!\mid p(n,r)\text{ for }r\leq u \implies u!\mid p(n+1,u)$$

# Principle of mathematical induction

## Induction on r

#### Base case

This is true for $r=1$ since $r!=1!=1\mid n$ for any $n\in\mathbb{N}$

#### Inductive Step

Let us assume that $r!\mid p(n,r)$ for $r\leq u$. Thus, we have to prove $(u+1)!\mid p(n,u+1)$.

Now, we do induction on $n$ to prove $(u+1)!\mid p(n,u+1)$. This is true for $n=1$ since $(u+1)!\mid p(1,u+1)=(u+1)!$. Suppose this is true for all $n\leq k$. Then, we have $(u+1)!\mid p(k,u+1)$ from result 1. Since, we assumed $r!\mid p(n,r)$ for $r\leq u$ and $(u+1)!\mid p(k,u+1)$, we have $r!\mid p(n,r)$ for $r\leq (u+1)$ and hence, $(u+1)!\mid p(k+1,u+1)$. Hence, by induction on $n$, we have $(u+1)!\mid p(n,u+1)$ for all $n\in\mathbb{N}$. This also completes our inductive step on $r$. Hence, $r!\mid p(n,r)$ for all $(n,r)\in\mathbb{N}\times\mathbb{N}$.


**Note:** Please see if the induction proof makes sense and if you can find a less cumbersome way of doing this proof.


## Induction on n

#### Base case

This is true for $n=1$ since $r!\mid 1\cdot2\cdot3\cdot\dots\cdot(1+r-1)=r!$ for any $r\in\mathbb{N}$.

#### Inductive Step

Let us assume that $r!\mid p(n,r)$ for $n\leq k$. Thus, we have to prove $r!\mid p(k+1,r)$.

Now, we do induction on $r$ to prove $r!\mid p(k+1,r)\forall r\in\mathbb{N}$. This is true for $r=1$ since $r!=1!=1\mid p(k+1,1)=(k+1)$. Now, let's assume that this is true for all $r\leq u$. Then, we have $u!\mid p(k+1,u)$ from result 2. Now, since $r\mid p(n,r)\forall n\leq (k+1)$ [as we assumed $r! \mid p(n,r)\forall n\leq k$ and hence $u!\mid p(n,u)\forall n\leq u$]. Thus, from result 1, $(u+1)!\mid p(k+1,u+1)$.

Hence, $r!\mid p(k+1,r)\forall r\in\mathbb{N}$. This also completes our induction step on $n$. Thus, $r!\mid p(n,r)\forall(n,r)\in\mathbb{N}\times\mathbb{N}$.

