---
title: "A GCD Proof"
date: 2023-10-01
difficulty: Intermediate
tags: ["Number Theory"]
concepts: ["GCD"]
equations:
  - $\left(\displaystyle\frac{a^n+b^n}{a+b},a+b\right)=(a+b,n)$
---

# Statement

Proof of $\left(\displaystyle\frac{a^n+b^n}{a+b},a+b\right)=(a+b,n)$ if $(a,b)=1$ and $n$ is an odd prime.

# Problem Statement

Prove that for $a,b\in\mathbb{Z}$ where $(a,b)=1$ and $n$ being an odd prime ($n>2$),
$$\left(\displaystyle\frac{a^n+b^n}{a+b},a+b\right)=(a+b,n)$$

# Proof

Let
$$\left(\displaystyle\frac{a^n+b^n}{a+b},a+b\right)=d$$
$$(a+b,n)=g$$
for $d,g\in\mathbb{Z}$ and $d,g>0$.

We have
$$
\begin{array}{rrl}
&a^n+b^n&=a^n+[(a+b)-a]^n\newline
&&=\bcancel{a^n}+(a+b)^n+\displaystyle\binom{n}{1}(a+b)^{n-1}(-a)+\dots+\displaystyle\binom{n}{n-2}(a+b)^2(-a)^{n-2}\newline
&&+\displaystyle\binom{n}{n-1}(a+b)(-a)^{n-1}+\bcancel{(-a)^n}\newline
\implies&\displaystyle\frac{a^n+b^n}{a+b}&=(a+b)^{n-1}+\displaystyle\binom{n}{1}(a+b)^{n-2}(-a)+\dots+\binom{n}{n-2}(a+b)(-a)^{n-2}+na^{n-1}\newline
\implies&\displaystyle\frac{a^n+b^n}{a+b}&=(a+b)k+na^{n-1}
\end{array}
$$
for $k\in\mathbb{Z}$


Now, since $d\mid\left(\displaystyle\frac{a^n+b^n}{a+b}\right)$ and $d\mid(a+b)$, we have
$$d\mid na^{n-1}$$
Also, since let $(a+b,a)=h$. Then, since $h\mid(a+b)$ and $h\mid a$, we have $h\mid(a+b)-a$ or $h\mid b$ or $h\mid(a,b)$. Since, $(a,b)=1$ and $h\mid (a,b)=1$ ($h>0$), we have $h=1$. Hence, $(a+b,a)=1$.


Thus, $\exists x,y\in\mathbb{Z}$ such that
$$(a+b)x+ay=1$$
from Bezout's identity.


Now, we have
$$[(a+b)x+ay]^{n-1}=1^{n-1}$$
$$
\begin{array}{rll}
\implies&[(a+b)x]^{n-1}+\displaystyle\binom{n-1}{1}[(a+b)x]^{n-2}(ay)+\dots&\newline
&\displaystyle\binom{n-1}{n-3}[(a+b)x]^{2}(ay)^{n-3}+\displaystyle\binom{n-1}{n-2}[(a+b)x]^{1}(ay)^{n-2}+ (ay)^{n-1}&=1\newline
\implies&(a+b)u+a^{n-1}v&=1\newline
\implies&(a+b)nu+a^{n-1}nv&=n
\end{array}
$$


Hence, for $r,v\in\mathbb{Z}$,
$$(a+b)r+[na^{n-1}]v=n$$
Now, since $d\mid (a+b)$ and $d\mid na^{n-1}$, we have
$$d\mid n$$
Thus, $d\mid(a+b)$ and $d\mid n$ $\implies$ $d\mid(a+b,n)$ or
$$d\mid g$$
Now, since
$$\displaystyle\frac{a^n+b^n}{a+b}=(a+b)k+na^{n-1}$$
if $g\mid(a+b)$ and $g\mid n$, then
$$g\mid\left(\displaystyle\frac{a^n+b^n}{a+b}\right)$$
or $g\mid\left(\displaystyle\frac{a^n+b^n}{a+b},a+b\right)$ or
$$g\mid d$$
Since $g,d>0$, we have $g=dp$ and $d=gq$ for some $p,q>0$ and $p,q\in\mathbb{Z}$. Hence, $d=gq=(dp)q=d(pq)$ or $pq=1$. Since $p,q>0$, we have $p=q=1$. Hence,
$$d=g$$
or
$$\left(\displaystyle\frac{a^n+b^n}{a+b},a+b\right)=(a+b,n)$$
Now since $n$ is a prime. If $n\mid (a+b)$, then $(a+b,n)=n$.


However, if $n\nmid (a+b)$, we have $(a+b)=nc+d$ for some $c,d\in\mathbb{Z}$ and $0<d<n$ (Euclid's Lemma). Suppose $(a+b,n)=t$. Then, since $t\mid(a+b)$ or $t\mid (nc+d)$ and $t\mid n$, we have $t\mid (nc+d)-n(c)$ or $t\mid d$. But if $(d,n)=1$ for $0<d<n$ since there is no divisor of $n$ other than $1$ and $n$. Hence, $t\mid(d,n)=1$ or $t\mid 1$. Thus,  $(a+b,n)=1$.
Hence, we have
$$
(a+b,n) = 
\begin{cases}
n,&\text{if $n\mid(a+b)$}\newline
1,&\text{if $n\nmid(a+b)$}
\end{cases}
$$
or
$$
\left(\displaystyle\frac{a^n+b^n}{a+b},a+b\right)=
\begin{cases}
n,&\text{if $n\mid(a+b)$}\newline
1,&\text{if $n\nmid(a+b)$}
\end{cases}
$$
